WIP: fibonacci reification

teaching/eutypes2018/sol/FibonacciReify.fst
@@ -53,16 +53,27 @@ effect St (a:Type) = STATE a (fun _ p -> forall x s1 . p (x,s1))
 let rec fibonacci_tot (n:nat) : Tot nat 
   = if n <= 1 then 1 else fibonacci_tot (n - 1) + fibonacci_tot (n - 2)
 
-let rec fibonacci (i:pos) (n:nat{n >= i}) : St unit (decreases (n - i)) = 
+let rec fibonacci (i:pos) : St unit = 
+  if i > 2 then (let temp = STATE?.get_right () in
+                 STATE?.put_right (STATE?.get_left () + STATE?.get_right ()); 
+                 STATE?.put_left temp;
+                 fibonacci (i - 1))
+
+(* let rec fibonacci (i:pos) (n:nat{n >= i}) : St unit (decreases (n - i)) = 
   if i < n then (let temp = STATE?.get_right () in
                  STATE?.put_right (STATE?.get_left () + STATE?.get_right ()); 
                  STATE?.put_left temp;
-                 fibonacci (i+1) n)
+                 fibonacci (i+1) n) *)
 
-let rec lemma_fibonacci (i:pos) (n:nat{n >= i})
+let lemma_fibonacci_two (i:pos) (m n:int)
+  : Lemma (requires (i <= 2))
+          (ensures  (let (_,(s,s')) = reify (fibonacci i) (m,n) in 
+                     s = m /\ s' = n))
+  = ()
+
+let rec lemma_fibonacci (i:pos) (m:pos)
   : Lemma (requires True)
-          (ensures (let (_,(s,s')) = reify (fibonacci i n) (1,1) in 
-                    s' = fibonacci_tot (n - i)))
-          (decreases (n - i))
-= if i = n then ()
-           else admit ()//; lemma_fibonacci (i+1) n
+          (ensures (let (_,(s,s')) = reify (fibonacci i) (fibonacci_tot m, fibonacci_tot (m + 1)) in 
+                    s  = fibonacci_tot (i + m - 2) /\ 
+                    s' = fibonacci_tot (i + m - 1)))
+= admit ()
